{
 "cells": [
  {
   "cell_type": "markdown",
   "id": "cd763a4f",
   "metadata": {},
   "source": [
    "### 题目（2）\n",
    "\n",
    "当 $1 \\le x \\le 2$ 时，化简：\n",
    "\n",
    "$$\n",
    "\\sqrt{x + 2\\sqrt{x - 1}} + \\sqrt{x - 2\\sqrt{x - 1}} = \\ ?\n",
    "$$\n",
    "\n",
    "---\n",
    "\n",
    "### 解法（平方法）：\n",
    "\n",
    "令：\n",
    "\n",
    "$$\n",
    "A = \\sqrt{x + 2\\sqrt{x - 1}} + \\sqrt{x - 2\\sqrt{x - 1}}\n",
    "$$\n",
    "\n",
    "对两边平方：\n",
    "\n",
    "$$\n",
    "A^2 = \\left( \\sqrt{x + 2\\sqrt{x - 1}} + \\sqrt{x - 2\\sqrt{x - 1}} \\right)^2\n",
    "$$\n",
    "\n",
    "展开平方：\n",
    "\n",
    "$$\n",
    "A^2 = (x + 2\\sqrt{x - 1}) + (x - 2\\sqrt{x - 1}) + 2 \\cdot \\sqrt{(x + 2\\sqrt{x - 1})(x - 2\\sqrt{x - 1})}\n",
    "$$\n",
    "\n",
    "化简前两项：\n",
    "\n",
    "$$\n",
    "A^2 = 2x + 2 \\cdot \\sqrt{x^2 - (2\\sqrt{x - 1})^2}\n",
    "= 2x + 2 \\cdot \\sqrt{x^2 - 4(x - 1)}\n",
    "= 2x + 2 \\cdot \\sqrt{x^2 - 4x + 4}\n",
    "$$\n",
    "\n",
    "注意：\n",
    "\n",
    "$$\n",
    "x^2 - 4x + 4 = (x - 2)^2\n",
    "$$\n",
    "\n",
    "又因为 $1 \\le x \\le 2$，所以：\n",
    "\n",
    "$$\n",
    "\\sqrt{(x - 2)^2} = 2 - x\n",
    "$$\n",
    "\n",
    "故：\n",
    "\n",
    "$$\n",
    "A^2 = 2x + 2(2 - x) = 2x + 4 - 2x = 4\n",
    "$$\n",
    "\n",
    "所以：\n",
    "\n",
    "$$\n",
    "A = \\sqrt{4} = 2\n",
    "$$\n",
    "\n",
    "---\n",
    "\n",
    "### 最终答案：\n",
    "\n",
    "$$\n",
    "\\boxed{2}\n",
    "$$\n"
   ]
  }
 ],
 "metadata": {
  "language_info": {
   "name": "python"
  }
 },
 "nbformat": 4,
 "nbformat_minor": 5
}
